theories/CompileCorrect.v
@@ -414,15 +414,15 @@ Qed.
 
 Opaque Malfunction.Int63.wB PArray.max_length.
 
-Lemma compile_correct `{Heap} Σ Σ' s t Γ Γ' h :
+Lemma compile_correct `{Heap} Σ Σ' s t Γ Γ' :
   (forall i mb ob, EGlobalEnv.lookup_inductive Σ i = Some (mb, ob) -> #|ob.(EAst.ind_ctors)| < Z.to_nat Malfunction.Int63.wB /\ forall n b, nth_error ob.(EAst.ind_ctors) n = Some b -> b.(EAst.cstr_nargs) < int_to_nat PArray.max_length) ->
   (forall na, Malfunction.Ident.Map.find na Γ' =  match lookup Γ na with Some v => compile_value Σ v | _ => fail "notfound" end) ->
   (forall c decl body v, EGlobalEnv.declared_constant Σ c decl -> EAst.cst_body decl = Some body -> EWcbvEvalNamed.eval Σ [] body v -> In ((Kernames.string_of_kername c), compile_value Σ v) Σ') ->
    EWcbvEvalNamed.eval Σ Γ s t ->
-   SemanticsSpec.eval Σ' Γ' h (compile Σ s) h (compile_value Σ t).
+   forall h, SemanticsSpec.eval Σ' Γ' h (compile Σ s) h (compile_value Σ t).
 Proof.
   rename H into HP; rename H0 into HH. 
-  intros Hextr HΓ HΣ Heval.
+  intros Hextr HΓ HΣ Heval h.
   revert Γ' HΓ.
   induction Heval; intros Γ_ HΓ; simp compile; try rewrite <- !compile_equation_1.
   - (* variables *)
